progress verifving pkae

secure_api/box/Box.AE.fst
@@ -20,65 +20,64 @@ let rec random_bytes n =
   | 0 -> let l:lbytes 0 = createL [] in l
   | _ -> append (createL [0x0buy]) (random_bytes (n-1))
 
-let leak #kl #rgn ip #i k =
+let leak #kl ip #i k =
  k.raw
 
 let getGT #kl #i k =
  k.raw
 
-let gen key_length #rgn ip i =
+let gen key_length ip i =
  Key (random_bytes key_length) true
 
-let coerce #key_length #rgn ip i raw =
+let coerce #key_length ip i raw =
   Key raw false
 
-let create_ae_key_package #rgn ip key_length =
-  KEY.create_key_package ip Flags.ae key_length (key key_length) (getGT #key_length) (leak #key_length #rgn ip) (gen key_length #rgn ip) (coerce ip)
+let create_ae_key_package ip key_length =
+  KEY.create_key_package ip Flags.ae key_length (key key_length) (getGT #key_length) (leak #key_length ip) (gen key_length ip) (coerce ip)
 
-let get_ap_pp #rgn #ip #key_length #kp #aparams ap = ap.pp
+let get_ap_pp #ip #key_length #kp #aparams ap = ap.pp
 
 //let get_ap_rgn #rgn #ip #key_length #kp #aparams ap = ap.log_rgn
 
-let recall_log #rgn #ip (#key_length:(n:nat{n<=32})) #kp #aparams ap = recall ap.log
+let recall_log #ip (#key_length:(n:nat{n<=32})) #kp #aparams ap = recall ap.log
 
-let get_ap_log #rgn #ip #key_length #kp #aparams ap = ap.log
+let get_log_rgn #ip #key_length #kp #aparams ap = ap.log_rgn
 
-let create_ae_package (#rgn:erid) ip (#key_length:(n:nat{n<=32})) kp aparams =
+let get_ap_log #ip #key_length #kp #aparams ap = ap.log
+
+let create_ae_package #ip (#key_length:(n:nat{n<=32})) (rgn:erid) kp aparams =
   let log_rgn = new_region rgn in
   let pp = PP Flags.ae aparams.scheme.valid_plain_length in
-  let log = MM.alloc #log_rgn #(message_log_key id aparams) #(message_log_range pp aparams) #(message_log_inv #pp #aparams) in
-  AE #rgn #ip #key_length #kp #aparams pp log_rgn log
+  let log = alloc_ae_message_log aparams log_rgn pp in
+  //let log = MM.alloc #log_rgn #(message_log_key aparams) #(message_log_range pp aparams) #(message_log_inv #pp #aparams) in
+  AE #ip #key_length #kp #aparams pp log_rgn log
 
 let zero_bytes valid_length n = Seq.create n (UInt8.uint_to_t 0)
 
 #set-options "--max_fuel 1 --max_ifuel 1 --z3rlimit 300"
-let encrypt #rgn #ip #i #key_length #kp #aparams ap k n p =
+let encrypt #ip #i #key_length #kp #aparams ap k n p =
   let honest_i = get_honesty ip i in
   let c =
     if honest_i && Flags.ae then
       aparams.scheme.enc_star (length p)
     else
       //lemma_dishonest_not_others
-<<<<<<< HEAD
-      aparams.scheme.enc (repr #rgn #ap.pp #ip p) k.raw n
-=======
-      aparams.scheme.enc (repr #rgn #ap.pp #ip #i p) k.raw n
->>>>>>> 264be060dd19c53ac9ab126eb69544c5fd13e723
+      aparams.scheme.enc (repr #ap.pp #ip #i p) k.raw n
   in
   recall ap.log;
-  MM.extend ap.log (LOG_KEY i n c) p;
+  MM.extend ap.log (i,n,c) p;
   c
 
-let decrypt #rgn #ip #i #key_length #kp #aparams ap k n c =
+let decrypt #ip #i #key_length #kp #aparams ap k n c =
   let honest_i = get_honesty ip i in
   match honest_i && Flags.ae with
   | true ->
-    (match MM.lookup ap.log (LOG_KEY i n c) with
+    (match MM.lookup ap.log (i,n,c) with
     | Some p ->
        recall ap.log;
        Some p
     | None -> None)
   | false ->
     match aparams.scheme.dec c k.raw n with
-    | Some p -> Some (Plain.coerce #rgn #ap.pp ip i p)
+    | Some p -> Some (Plain.coerce #ap.pp ip i p)
     | None -> None
