secure_api/box/Box.AE.fsti
@@ -9,10 +9,12 @@ open FStar.Endianness
 
 open Box.Plain
 open Box.Index
+open Mem
 
 module KEY = Box.Key
 module Flags = Box.Flags
 module MM = FStar.Monotonic.Map
+
 
 // KEY Package definition
 
@@ -27,15 +29,15 @@ noeq abstract type key (key_length:(n:nat{n<=32})) (i:inst_id) =
        h:bool ->
        key key_length i
 
-val leak: #key_length:(n:nat{n<=32}) -> #rgn:erid -> ip:index_package rgn -> #i:inst_id{~Flags.ae \/ dishonest ip i} -> k:key key_length i -> raw:lbytes key_length{raw = k.raw}
+val leak: #key_length:(n:nat{n<=32}) -> ip:index_package -> #i:inst_id{~Flags.ae \/ dishonest ip i} -> k:key key_length i -> raw:lbytes key_length{raw = k.raw}
 
 val getGT: #key_length:(n:nat{n<=32}) -> #i:inst_id -> k:key key_length i -> GTot (raw:lbytes key_length{raw = k.raw})
 
-val gen: key_length:(n:nat{n<=32}) -> #rgn:erid -> ip:index_package rgn -> i:inst_id -> k:key key_length i
+val gen: key_length:(n:nat{n<=32}) -> ip:index_package -> i:inst_id -> k:key key_length i
 
-val coerce: #key_length:(n:nat{n<=32}) -> #rgn:erid -> ip:index_package rgn -> i:inst_id{~Flags.ae \/ dishonest ip i} -> raw:lbytes key_length -> k:key key_length i{k.raw = raw}
+val coerce: #key_length:(n:nat{n<=32}) -> ip:index_package -> i:inst_id{~Flags.ae \/ dishonest ip i} -> raw:lbytes key_length -> k:key key_length i{k.raw = raw}
 
-val create_ae_key_package: #rgn:erid -> ip:index_package rgn -> key_length:(n:nat{n<=32}) -> KEY.key_package ip key_length (key key_length)
+val create_ae_key_package: ip:index_package -> key_length:(n:nat{n<=32}) -> KEY.key_package ip key_length (key key_length)
 
 
 // Definition AE package
@@ -54,7 +56,7 @@ noeq type encryption_scheme (key_length:(n:nat{n<=32})) (nonce_length:(n:nat{n<=
 //      Some? dec_result
 //      /\ Some?.v dec_result == p
 //    ))
-//    ) ->
+      //    ) ->
     encryption_scheme key_length nonce_length
 
 // Make them abstract or move the flag to ae_package?
@@ -69,73 +71,83 @@ noeq type ae_parameters =
 let nonce (aparams:ae_parameters) = lbytes aparams.nonce_length
 let ciphertext (aparams:ae_parameters) = c:bytes32{aparams.scheme.valid_cipher_length (Seq.length c)}
 
-type message_log_key (id:eqtype) (aparams:ae_parameters) =
-  | LOG_KEY: i:inst_id -> n:nonce aparams -> c:ciphertext aparams -> message_log_key id aparams
+let fst t = Mktuple3?._1 t
+let snd t = Mktuple3?._2 t
+let thrd t = Mktuple3?._3 t
 
-let message_log_value (i:inst_id) (pp:plain_package) = protected_plain pp i
-let message_log_range (pp:plain_package) (aparams:ae_parameters) (k:message_log_key id aparams) = message_log_value (k.i) pp
-let message_log_inv (#pp:plain_package) (#aparams:ae_parameters) (f:MM.map' (message_log_key id aparams) (message_log_range pp aparams)) = True
+//type message_log_key (aparams:ae_parameters) = inst_id*nonce aparams*ciphertext aparams
+////  | LOG_KEY: i:inst_id -> n:nonce aparams -> c:ciphertext aparams -> message_log_key aparams
+//
+//let message_log_value (pp:plain_package) (i:inst_id) = protected_plain pp i
+//let message_log_range (pp:plain_package) (aparams:ae_parameters) (k:message_log_key aparams) = message_log_value pp (Mktuple3?._1 k)
+//let message_log_inv (#pp:plain_package) (#aparams:ae_parameters) (f:MM.map' (message_log_key aparams) (message_log_range pp aparams)) = True
+//
+//let message_log (#pp:plain_package) (rgn:erid) (aparams:ae_parameters) =
+//  MM.t rgn (message_log_key aparams) (message_log_range pp aparams) (message_log_inv)
+//
+//let empty_message_log (aparams:ae_parameters) (pp:plain_package) = MM.empty_map (message_log_key aparams) (message_log_range pp aparams)
 
-let message_log (#pp:plain_package) (rgn:erid) (aparams:ae_parameters) =
-  MM.t rgn (message_log_key id aparams) (message_log_range pp aparams) (message_log_inv)
+let ae_message_log (aparams:ae_parameters) = Mem.message_log (nonce aparams) (ciphertext aparams)
+let empty_ae_message_log (aparams:ae_parameters) = Mem.empty_message_log (nonce aparams) (ciphertext aparams)
+let alloc_ae_message_log (aparams:ae_parameters) = Mem.alloc_message_log (nonce aparams) (ciphertext aparams)
 
-let empty_message_log (aparams:ae_parameters) (pp:plain_package) = MM.empty_map (message_log_key id aparams) (message_log_range pp aparams)
-
-noeq abstract type ae_package (#rgn:erid) (#ip:index_package rgn) (#key_length:(n:nat{n<=32})) (kp:KEY.key_package ip key_length (key key_length)) (aparams:ae_parameters{aparams.keylength = key_length}) =
+noeq abstract type ae_package (#ip:index_package) (#key_length:(n:nat{n<=32})) (kp:KEY.key_package ip key_length (key key_length)) (aparams:ae_parameters{aparams.keylength = key_length}) =
   | AE:
     pp:plain_package{pp == PP Flags.ae aparams.scheme.valid_plain_length} ->
-    log_rgn:erid{extends log_rgn rgn} ->
-    log:message_log #pp log_rgn aparams ->
-    ae_package #rgn #ip #key_length kp aparams
+    log_rgn:erid ->
+    log:ae_message_log aparams pp log_rgn ->
+    ae_package #ip #key_length kp aparams
 
-//val get_flag: (#rgn:erid) -> (#ip:index_package rgn) -> (#key_length:(n:nat{n<=32})) -> (#kp:KEY.key_package ip key_length (key key_length)) -> (#aparams:ae_parameters{aparams.keylength = key_length}) -> ap:ae_package kp aparams -> GTot (b:bool{b = ap.b})
+//val get_flag: (#ip:index_package rgn) -> (#key_length:(n:nat{n<=32})) -> (#kp:KEY.key_package ip key_length (key key_length)) -> (#aparams:ae_parameters{aparams.keylength = key_length}) -> ap:ae_package kp aparams -> GTot (b:bool{b = ap.b})
 //let valid_ae_plain_package (aparams:ae_parameters) (pp:plain_package) = pp == PP (get_ae_flagGT aparams) aparams.scheme.valid_plain_length
 
-val get_ap_pp: (#rgn:erid) -> (#ip:index_package rgn) -> (#key_length:(n:nat{n<=32})) -> (#kp:KEY.key_package ip key_length (key key_length)) -> (#aparams:ae_parameters{aparams.keylength = key_length}) -> (ap:ae_package #rgn #ip #key_length kp aparams) -> pp:plain_package{pp == PP Flags.ae aparams.scheme.valid_plain_length /\ pp == ap.pp}
+val get_ap_pp: (#ip:index_package) -> (#key_length:(n:nat{n<=32})) -> (#kp:KEY.key_package ip key_length (key key_length)) -> (#aparams:ae_parameters{aparams.keylength = key_length}) -> (ap:ae_package #ip #key_length kp aparams) -> pp:plain_package{pp.flag == Flags.ae /\ pp.valid_length == aparams.scheme.valid_plain_length /\ pp == ap.pp}
 
-//val get_ap_rgn: (#rgn:erid) -> (#ip:index_package rgn) -> (#key_length:(n:nat{n<=32})) -> (#kp:KEY.key_package ip key_length (key key_length)) -> (#aparams:ae_parameters{aparams.keylength = key_length}) -> (ap:ae_package #rgn #ip #key_length kp aparams) -> rgn:erid{rgn = ap.rgn}
+//val get_ap_rgn: (#ip:index_package rgn) -> (#key_length:(n:nat{n<=32})) -> (#kp:KEY.key_package ip key_length (key key_length)) -> (#aparams:ae_parameters{aparams.keylength = key_length}) -> (ap:ae_package #rgn #ip #key_length kp aparams) -> rgn:erid{rgn = ap.rgn}
 
-val recall_log: (#rgn:erid) -> (#ip:index_package rgn) -> (#key_length:(n:nat{n<=32})) -> (#kp:KEY.key_package ip key_length (key key_length)) -> (#aparams:ae_parameters{aparams.keylength = key_length}) -> (ap:ae_package kp aparams) -> ST unit
+val recall_log: (#ip:index_package) -> (#key_length:(n:nat{n<=32})) -> (#kp:KEY.key_package ip key_length (key key_length)) -> (#aparams:ae_parameters{aparams.keylength = key_length}) -> (ap:ae_package kp aparams) -> ST unit
   (requires (fun h0 -> True))
   (ensures (fun h0 _ h1 ->
     h0 == h1
     /\ contains h1 ap.log
   ))
 
-val get_ap_log: (#rgn:erid) -> (#ip:index_package rgn) -> (#key_length:(n:nat{n<=32})) -> (#kp:KEY.key_package ip key_length (key key_length)) -> (#aparams:ae_parameters{aparams.keylength = key_length}) -> (ap:ae_package kp aparams) -> GTot (message_log #ap.pp ap.log_rgn aparams)
+val get_log_rgn: (#ip:index_package) -> (#key_length:(n:nat{n<=32})) -> (#kp:KEY.key_package ip key_length (key key_length)) -> (#aparams:ae_parameters{aparams.keylength = key_length}) -> (ap:ae_package kp aparams) -> Tot (rgn:erid{rgn = ap.log_rgn})
 
-let nonce_is_unique (#rgn:erid) (#ip:index_package rgn) (#key_length:(n:nat{n<=32})) (#kp:KEY.key_package ip key_length (key key_length)) (#aparams:ae_parameters{aparams.keylength = key_length}) (ap:ae_package kp aparams) (i:inst_id) (n:nonce aparams) (h0:mem) =
-  forall c . MM.fresh ap.log (LOG_KEY i n c) h0
+val get_ap_log: (#ip:index_package) -> (#key_length:(n:nat{n<=32})) -> (#kp:KEY.key_package ip key_length (key key_length)) -> (#aparams:ae_parameters{aparams.keylength = key_length}) -> (ap:ae_package kp aparams) -> GTot (ae_message_log  aparams (get_ap_pp ap) (get_log_rgn ap))
 
-val create_ae_package: (#rgn:erid) -> (ip:index_package rgn) -> (#key_length:(n:nat{n<=32})) -> (kp:KEY.key_package ip key_length (key key_length)) -> (aparams:ae_parameters{aparams.keylength = key_length}) -> ST (ae_package kp aparams)
+let nonce_is_unique (#ip:index_package) (#key_length:(n:nat{n<=32})) (#kp:KEY.key_package ip key_length (key key_length)) (#aparams:ae_parameters{aparams.keylength = key_length}) (ap:ae_package kp aparams) (i:inst_id) (n:nonce aparams) (h0:mem) =
+  forall c . MM.fresh ap.log (i,n,c) h0
+
+val create_ae_package: (#ip:index_package) -> (#key_length:(n:nat{n<=32})) -> (rgn:erid) -> (kp:KEY.key_package ip key_length (key key_length)) -> (aparams:ae_parameters{aparams.keylength = key_length}) -> ST (ae_package kp aparams)
   (requires (fun h0 -> True))
   (ensures (fun h0 ap h1 ->
     modifies (Set.singleton rgn) h0 h1
     /\ (forall n i . nonce_is_unique ap i n h1)
     /\ extends ap.log_rgn rgn
     /\ contains h1 ap.log
-    /\ sel h1 ap.log == empty_message_log aparams ap.pp
+    /\ sel h1 ap.log == empty_ae_message_log aparams ap.pp
   ))
 
 val zero_bytes: (valid_length:(n:n32 -> bool)) -> (n:n32{valid_length n}) -> p:lbytes n{valid_length (Seq.length p)}
 
-let encrypt_modified_regions (#rgn:erid) (#ip:index_package rgn) (#key_length:(n:nat{n<=32})) (#kp:KEY.key_package ip key_length (key key_length)) (#aparams:ae_parameters{aparams.keylength = key_length}) (ap:ae_package kp aparams) : (Set.set rid) = Set.singleton ap.log_rgn
+let encrypt_modified_regions (#ip:index_package) (#key_length:(n:nat{n<=32})) (#kp:KEY.key_package ip key_length (key key_length)) (#aparams:ae_parameters{aparams.keylength = key_length}) (ap:ae_package kp aparams) : (Set.set rid) = Set.singleton ap.log_rgn
 
-let encrypt_log_change (#rgn:erid) (#ip:index_package rgn) (#key_length:(n:nat{n<=32})) (#kp:KEY.key_package ip key_length (key key_length)) (#aparams:ae_parameters{aparams.keylength = key_length}) (ap:ae_package kp aparams) (i:inst_id) (n:nonce aparams) (c:ciphertext aparams) (p:protected_plain ap.pp i) (h0:mem) (h1:mem) =
+let encrypt_log_change (#ip:index_package) (#key_length:(n:nat{n<=32})) (#kp:KEY.key_package ip key_length (key key_length)) (#aparams:ae_parameters{aparams.keylength = key_length}) (ap:ae_package kp aparams) (i:inst_id) (n:nonce aparams) (c:ciphertext aparams) (p:protected_plain ap.pp i) (h0:mem) (h1:mem) =
     let a = 1 in
-    witnessed (MM.contains ap.log (LOG_KEY i n c) p)
+    witnessed (MM.contains ap.log (i,n,c) p)
     /\ contains h0 ap.log
-    /\ sel h1 ap.log == MM.upd (sel h0 ap.log) (LOG_KEY i n c) p
+    /\ sel h1 ap.log == MM.upd (sel h0 ap.log) (i,n,c) p
 
-let encrypt_functional_spec (#rgn:erid) (#ip:index_package rgn) (#i:inst_id) (#key_length:(n:nat{n<=32})) (#kp:KEY.key_package ip key_length (key key_length)) (#aparams:ae_parameters{aparams.keylength = key_length}) (ap:ae_package kp aparams) (k:key key_length i) (n:nonce aparams) (c:ciphertext aparams) (p:protected_plain ap.pp i) =
+let encrypt_functional_spec (#ip:index_package) (#i:inst_id) (#key_length:(n:nat{n<=32})) (#kp:KEY.key_package ip key_length (key key_length)) (#aparams:ae_parameters{aparams.keylength = key_length}) (ap:ae_package kp aparams) (k:key key_length i) (n:nonce aparams) (c:ciphertext aparams) (p:protected_plain ap.pp i) =
   let a = 1 in
   ((honest ip i /\ Flags.ae) ==>
     (c = aparams.scheme.enc_star (length p)))
   /\ ((dishonest ip i \/ ~Flags.ae) ==>
-    (c = aparams.scheme.enc (repr #rgn #ap.pp #ip #i p) k.raw n))
+    (c = aparams.scheme.enc (repr #ap.pp #ip #i p) k.raw n))
 
 #set-options "--max_fuel 1 --max_ifuel 1 --z3rlimit 300"
-val encrypt: #rgn:erid -> #ip:index_package rgn -> #i:inst_id -> #key_length:(n:nat{n<=32}) -> #kp:KEY.key_package ip key_length (key key_length) -> #aparams:ae_parameters{key_length = aparams.keylength} -> ap:ae_package kp aparams -> k:key key_length i -> n:nonce aparams -> p:protected_plain ap.pp i -> ST (ciphertext aparams)
+val encrypt: #ip:index_package -> #i:inst_id -> #key_length:(n:nat{n<=32}) -> #kp:KEY.key_package ip key_length (key key_length) -> #aparams:ae_parameters{key_length = aparams.keylength} -> ap:ae_package kp aparams -> k:key key_length i -> n:nonce aparams -> p:protected_plain ap.pp i -> ST (ciphertext aparams)
   (requires (fun h0 ->
     (nonce_is_unique ap i n h0)
     /\ registered ip i
@@ -147,14 +159,13 @@ val encrypt: #rgn:erid -> #ip:index_package rgn -> #i:inst_id -> #key_length:(n:
     /\ ((forall n'. nonce_is_unique ap i n' h0) ==> (forall n' . n' =!=n ==> nonce_is_unique ap i n' h1))
   ))
 
-let decrypt_modified_regions (#rgn:erid) (#ip:index_package rgn) (#key_length:(n:nat{n<=32})) (#kp:KEY.key_package ip key_length (key key_length)) (#aparams:ae_parameters{aparams.keylength = key_length}) (ap:ae_package kp aparams) = Set.empty
+let decrypt_modified_regions (#ip:index_package) (#key_length:(n:nat{n<=32})) (#kp:KEY.key_package ip key_length (key key_length)) (#aparams:ae_parameters{aparams.keylength = key_length}) (ap:ae_package kp aparams) = Set.empty
 
-let decrypt_log_change (#rgn:erid) (#ip:index_package rgn) (#key_length:(n:nat{n<=32})) (#kp:KEY.key_package ip key_length (key key_length)) (#aparams:ae_parameters{aparams.keylength = key_length}) (ap:ae_package kp aparams) (h0:mem) (h1:mem) =
+let decrypt_log_change (#ip:index_package) (#key_length:(n:nat{n<=32})) (#kp:KEY.key_package ip key_length (key key_length)) (#aparams:ae_parameters{aparams.keylength = key_length}) (ap:ae_package kp aparams) (h0:mem) (h1:mem) =
   sel h1 ap.log == sel h0 ap.log
 
 
-let decrypt_functional_spec (#rgn:erid)
-                            (#ip:index_package rgn)
+let decrypt_functional_spec (#ip:index_package)
                             (#i:inst_id)
                             (#key_length:(n:nat{n<=32}))
                             (#kp:KEY.key_package ip key_length (key key_length))
@@ -168,8 +179,8 @@ let decrypt_functional_spec (#rgn:erid)
   let a = 1 in
     ((honest ip i /\ Flags.ae) ==>
       (match p with
-       | Some p' -> MM.contains ap.log (LOG_KEY i n c) p' h0
-       | None -> MM.fresh ap.log (LOG_KEY i n c) h0
+       | Some p' -> MM.contains ap.log (i,n,c) p' h0
+       | None -> MM.fresh ap.log (i,n,c) h0
       ))
     /\ ((dishonest ip i \/ ~Flags.ae) ==>
       (match aparams.scheme.dec c k.raw n with
@@ -177,7 +188,7 @@ let decrypt_functional_spec (#rgn:erid)
        | None -> None? p
       ))
 
-val decrypt: #rgn:erid -> #ip:index_package rgn -> #i:inst_id -> #key_length:(n:nat{n<=32}) -> #kp:KEY.key_package ip key_length (key key_length) -> #aparams:ae_parameters{key_length = aparams.keylength} -> ap:ae_package kp aparams -> k:key key_length i -> n:nonce aparams -> c:ciphertext aparams -> ST (option (p:protected_plain ap.pp i))
+val decrypt: #ip:index_package -> #i:inst_id -> #key_length:(n:nat{n<=32}) -> #kp:KEY.key_package ip key_length (key key_length) -> #aparams:ae_parameters{key_length = aparams.keylength} -> ap:ae_package kp aparams -> k:key key_length i -> n:nonce aparams -> c:ciphertext aparams -> ST (option (p:protected_plain ap.pp i))
   (requires (fun h0 ->
     registered ip i
   ))
