secure_api/box/Box.Key.fst
@@ -7,19 +7,18 @@ open FStar.Endianness
 open Box.Index
 
 // Definition KEY package
-noeq type key_package (#rgn:erid) (ip:index_package rgn) (key_length:(n:nat{n<=32})) (key_type:(inst_id  -> Type0)) =
+noeq type key_package (ip:index_package) (key_length:(n:nat{n<=32})) (key_type:(inst_id  -> Type0)) =
   | KP:
   flag: Type0 ->
   getGT: (#i:inst_id -> k:key_type i -> GTot (lbytes key_length)) ->
   leak: (#i:inst_id{dishonest ip i \/ ~flag} -> k:key_type i -> (raw:lbytes key_length{raw = getGT k})) ->
   gen: (i:inst_id -> k:key_type i) ->
   coerce: (i:inst_id{~flag \/ dishonest ip i} -> raw:lbytes key_length -> (k:key_type i{raw = getGT k})) ->
-  key_package #rgn ip key_length key_type
+  key_package ip key_length key_type
 
 #set-options "--z3rlimit 300 --max_ifuel 1 --max_fuel 0"
 val create_key_package:
-  (#rgn:erid) ->
-  (ip:index_package rgn) ->
+  (ip:index_package) ->
   (flag:Type0) ->
   (key_length:(n:nat{n<=32})) ->
   (key_type:(inst_id -> Type0)) ->
@@ -27,7 +26,7 @@ val create_key_package:
   (param_leak: (#i:inst_id{dishonest ip i \/ ~flag} -> k:key_type i -> (raw:lbytes key_length{raw = param_getGT k}))) ->
   (param_gen: (i:inst_id -> k:key_type i)) ->
   (param_coerce: (i:inst_id{dishonest ip i \/ ~flag} -> raw:lbytes key_length -> (k:key_type i{raw = param_getGT k}))) ->
-  (kp:key_package #rgn ip key_length key_type{True
+  (kp:key_package ip key_length key_type{True
 //    param_hon == hon kp
 //    /\ param_hon == kp.hon
 //    /\ param_getGT == kp.getGT
@@ -36,5 +35,5 @@ val create_key_package:
 //    /\ param_gen == gen kp
 //    /\ param_cset == cset kp
   })
-let create_key_package #rgn ip flag key_length key_type getGT leak gen coerce =
+let create_key_package ip flag key_length key_type getGT leak gen coerce =
   KP flag getGT leak gen coerce
