secure_api/box/Box.ODH.fst
@@ -22,7 +22,10 @@ let get_share_raw #oparams sh = sh.raw_sh
 
 let get_exponent_raw #oparams exp = exp.raw_exp
 
-let gen_dh #rgn ip oparam =
+let gen_dh_footprint ip oparams h0 h1 =
+  register_footprint ip h0 h1
+
+let gen_dh ip oparam =
   let raw_exp = random_bytes oparam.exponent_length in
   let raw_sh = oparam.exponentiate raw_exp oparam.generator in
   let h0 = get() in
@@ -31,30 +34,36 @@ let gen_dh #rgn ip oparam =
   let sh = SH raw_sh in
   (EXP raw_exp sh,sh)
 
-let coerce_dh_sh #rgn ip oparam raw_sh =
+let coerce_dh_sh_footprint ip oparams raw_sh h0 h1 =
+  register_footprint ip h0 h1
+
+let coerce_dh_sh ip oparam raw_sh =
   register ip (PK_id raw_sh) false;
   SH raw_sh
 
-let coerce_dh_exp #rgn ip oparam raw_exp =
+let coerce_dh_exp_footprint ip oparams raw_sh h0 h1 =
+  register_footprint ip h0 h1
+
+let coerce_dh_exp ip oparam raw_exp =
   let raw_sh = oparam.exponentiate raw_exp oparam.generator in
   register ip (PK_id raw_sh) false;
   let sh = SH raw_sh in
   EXP raw_exp sh
 
-let get_op_rgn #rgn #ip #key_length #key_type #kp #oparam op = op.kp_log_rgn
+let get_op_rgn #ip #key_length #key_type #kp #oparam op = op.kp_log_rgn
 
-let get_op_log #rgn #ip #key_length #key_type #kp #oparam op = op.kp_log
+let get_op_log #ip #key_length #key_type #kp #oparam op = op.kp_log
 
-let recall_op_log #rgn #ip #key_length #key_type #kp #oparam op =
+let recall_op_log #ip #key_length #key_type #kp #oparam op =
   recall op.kp_log
 
-let create_odh_package #rgn #ip #key_length #key_type kp oparam =
+let create_odh_package #ip #key_length #key_type rgn kp oparam =
   let odh_rgn = new_region rgn in
   let kp_log = MM.alloc #odh_rgn #key_package_log_key #(key_package_log_range key_type) #(key_package_log_inv key_type) in
   ODH odh_rgn kp_log
 
 #set-options "--z3rlimit 300 --max_ifuel 2 --max_fuel 1"
-let dh_op #rgn #ip #key_length #key_type #kp #oparam op sh exp =
+let dh_op #ip #key_length #key_type #kp #oparam op sh exp =
   let i = compose_id (PK_id sh.raw_sh) (PK_id exp.sh.raw_sh) in
   let both_honest = get_honesty ip i in
     if Flags.prf_odh && both_honest then
