secure_api/box/Box.ODH.fsti
@@ -47,25 +47,32 @@ val get_share_raw: #oparams:odh_parameters -> sh:share oparams -> raw:lbytes opa
 
 val get_exponent_raw: #oparams:odh_parameters -> exp:exponent oparams -> GTot (raw:lbytes oparams.exponent_length{raw = exp.raw_exp})
 
-val gen_dh: (#rgn:erid) -> (ip:index_package rgn) -> (oparam:odh_parameters) -> ST (dh_keypair:(exponent oparam*share oparam){(fst dh_keypair).sh=snd dh_keypair})
+val gen_dh_footprint: ip:index_package -> oparam:odh_parameters -> h0:mem -> h1:mem -> Type0
+
+val gen_dh: (ip:index_package) -> (oparam:odh_parameters) -> ST (dh_keypair:(exponent oparam*share oparam))
   (requires (fun h0 -> True))
   (ensures (fun h0 (e,sh) h1 ->
-    registered ip (PK_id sh.raw_sh)
+    e.sh == sh
+    /\ registered ip (PK_id sh.raw_sh)
     /\ honest ip (PK_id sh.raw_sh)
-    /\ register_footprint ip h0 h1
+    /\ gen_dh_footprint ip oparam h0 h1
   ))
 
-val coerce_dh_sh: (#rgn:erid) -> (ip:index_package rgn) -> (oparam:odh_parameters) -> (raw_sh:lbytes oparam.share_length) -> ST (sh:share oparam{sh.raw_sh = raw_sh})
+val coerce_dh_sh_footprint: (ip:index_package) -> (oparam:odh_parameters) -> (raw_sh:lbytes oparam.share_length) -> h0:mem -> h1:mem -> Type0
+
+val coerce_dh_sh: (ip:index_package) -> (oparam:odh_parameters) -> (raw_sh:lbytes oparam.share_length) -> ST (sh:share oparam{sh.raw_sh = raw_sh})
   (requires (fun h0 ->
     fresh ip (PK_id raw_sh) h0
   ))
   (ensures (fun h0 sh h1 ->
     registered ip (PK_id raw_sh)
     /\ dishonest ip (PK_id raw_sh)
-    /\ register_footprint ip h0 h1
+    /\ coerce_dh_sh_footprint ip oparam raw_sh h0 h1
   ))
 
-val coerce_dh_exp: (#rgn:erid) -> (ip:index_package rgn) -> (oparam:odh_parameters) -> (raw_exp:lbytes oparam.exponent_length) -> ST (exp:exponent oparam{exp.raw_exp = raw_exp})
+val coerce_dh_exp_footprint: (ip:index_package) -> (oparam:odh_parameters) -> (raw_exp:lbytes oparam.exponent_length) -> h0:mem -> h1:mem -> Type0
+
+val coerce_dh_exp: (ip:index_package) -> (oparam:odh_parameters) -> (raw_exp:lbytes oparam.exponent_length) -> ST (exp:exponent oparam{exp.raw_exp = raw_exp})
   (requires (fun h0 ->
     let raw_sh = oparam.exponentiate raw_exp oparam.generator in
     fresh ip (PK_id raw_sh) h0
@@ -74,42 +81,42 @@ val coerce_dh_exp: (#rgn:erid) -> (ip:index_package rgn) -> (oparam:odh_paramete
     let raw_sh = oparam.exponentiate raw_exp oparam.generator in
     registered ip (PK_id raw_sh)
     /\ dishonest ip (PK_id raw_sh)
-    /\ register_footprint ip h0 h1
+    /\ coerce_dh_exp_footprint ip oparam raw_exp h0 h1
   ))
 
-let key_package_log_key = id
-let key_package_log_value (i:id) (key_type:(id -> Type0)) = key_type i
-let key_package_log_range  (key_type:(id -> Type0)) (k:key_package_log_key) = key_package_log_value k key_type
-let key_package_log_inv (key_type:(id -> Type0)) (f:MM.map' (key_package_log_key) (key_package_log_range key_type)) = True
+let key_package_log_key = inst_id
+let key_package_log_value (i:inst_id) (key_type:(inst_id -> Type0)) = key_type i
+let key_package_log_range  (key_type:(inst_id -> Type0)) (k:key_package_log_key) = key_package_log_value k key_type
+let key_package_log_inv (key_type:(inst_id -> Type0)) (f:MM.map' (key_package_log_key) (key_package_log_range key_type)) = True
 
-let key_package_log (rgn:erid) (key_type:(id -> Type0)) =
+let key_package_log (rgn:erid) (key_type:(inst_id -> Type0)) =
   MM.t rgn (key_package_log_key) (key_package_log_range key_type) (key_package_log_inv key_type)
 
-noeq abstract type odh_package (#rgn:erid) (#ip:index_package rgn) (#key_length:(n:nat{n<=32})) (#key_type:(id -> Type0)) (kp:key_package ip key_length key_type) (oparam:odh_parameters{oparam.hash_length = key_length}) =
+noeq abstract type odh_package (#ip:index_package) (#key_length:(n:nat{n<=32})) (#key_type:(inst_id -> Type0)) (kp:key_package ip key_length key_type) (oparam:odh_parameters{oparam.hash_length = key_length}) =
   | ODH:
-  kp_log_rgn:erid{extends kp_log_rgn rgn} ->
+  kp_log_rgn:erid ->
   kp_log:key_package_log kp_log_rgn key_type ->
-  odh_package #rgn #ip #key_length #key_type kp oparam
+  odh_package #ip #key_length #key_type kp oparam
 
-val get_op_rgn: (#rgn:erid) -> (#ip:index_package rgn) -> (#key_length:(n:nat{n<=32})) -> (#key_type:(id -> Type0)) -> (#kp:key_package ip key_length key_type) -> (#oparam:odh_parameters{oparam.hash_length = key_length}) -> op:odh_package kp oparam -> (rgn:erid{rgn = op.kp_log_rgn})
+val get_op_rgn: (#ip:index_package) -> (#key_length:(n:nat{n<=32})) -> (#key_type:(inst_id -> Type0)) -> (#kp:key_package ip key_length key_type) -> (#oparam:odh_parameters{oparam.hash_length = key_length}) -> op:odh_package kp oparam -> (rgn:erid{rgn = op.kp_log_rgn})
 
-val get_op_log: (#rgn:erid) -> (#ip:index_package rgn) -> (#key_length:(n:nat{n<=32})) -> (#key_type:(id -> Type0)) -> (#kp:key_package ip key_length key_type) -> (#oparam:odh_parameters{oparam.hash_length = key_length}) -> op:odh_package kp oparam -> GTot (log:key_package_log op.kp_log_rgn key_type)
+val get_op_log: (#ip:index_package) -> (#key_length:(n:nat{n<=32})) -> (#key_type:(inst_id -> Type0)) -> (#kp:key_package ip key_length key_type) -> (#oparam:odh_parameters{oparam.hash_length = key_length}) -> op:odh_package kp oparam -> GTot (log:key_package_log op.kp_log_rgn key_type)
 
-val recall_op_log: (#rgn:erid) -> (#ip:index_package rgn) -> (#key_length:(n:nat{n<=32})) -> (#key_type:(id -> Type0)) -> (#kp:key_package ip key_length key_type) -> (#oparam:odh_parameters{oparam.hash_length = key_length}) -> op:odh_package kp oparam -> ST unit
+val recall_op_log: (#ip:index_package) -> (#key_length:(n:nat{n<=32})) -> (#key_type:(inst_id -> Type0)) -> (#kp:key_package ip key_length key_type) -> (#oparam:odh_parameters{oparam.hash_length = key_length}) -> op:odh_package kp oparam -> ST unit
   (requires (fun h0 -> True))
   (ensures (fun h0 _ h1 ->
     h0 == h1
     /\ contains h1 op.kp_log
   ))
 
-val create_odh_package: (#rgn:erid) -> (#ip:index_package rgn) -> (#key_length:(n:nat{n<=32})) -> (#key_type:(id -> Type0)) -> (kp:key_package ip key_length key_type) -> (oparam:odh_parameters{oparam.hash_length = key_length}) -> ST (odh_package #rgn #ip #key_length #key_type kp oparam)
+val create_odh_package: (#ip:index_package) -> (#key_length:(n:nat{n<=32})) -> (#key_type:(inst_id -> Type0)) -> (rgn:erid) -> (kp:key_package ip key_length key_type) -> (oparam:odh_parameters{oparam.hash_length = key_length}) -> ST (odh_package #ip #key_length #key_type kp oparam)
   (requires (fun h0 -> True))
   (ensures (fun h0 op h1 ->
     modifies (Set.singleton op.kp_log_rgn) h0 h1
     /\ extends op.kp_log_rgn rgn
   ))
 
-let dh_op_memory_footprint (#rgn:erid) (#ip:index_package rgn) (#key_length:(n:nat{n<=32})) (#key_type:(id -> Type0)) (#kp:key_package ip key_length key_type) (#oparam:odh_parameters{oparam.hash_length = key_length}) (op:odh_package kp oparam) (sh:share oparam) (exp:exponent oparam{exp.sh.raw_sh <> sh.raw_sh}) (h0:mem) (h1:mem) =
+let dh_op_memory_footprint (#ip:index_package) (#key_length:(n:nat{n<=32})) (#key_type:(inst_id -> Type0)) (#kp:key_package ip key_length key_type) (#oparam:odh_parameters{oparam.hash_length = key_length}) (op:odh_package kp oparam) (sh:share oparam) (exp:exponent oparam{exp.sh.raw_sh <> sh.raw_sh}) (h0:mem) (h1:mem) =
   let i = compose_id (PK_id sh.raw_sh) (PK_id exp.sh.raw_sh) in
   let both_honest = honest ip i in
   ((both_honest /\ Flags.prf_odh) ==>
@@ -121,7 +128,7 @@ let dh_op_memory_footprint (#rgn:erid) (#ip:index_package rgn) (#key_length:(n:n
   /\ ((~both_honest \/ ~Flags.prf_odh) ==>
       modifies Set.empty h0 h1)
 
-let dh_op_log_change (#rgn:erid) (#ip:index_package rgn) (#key_length:(n:nat{n<=32})) (#key_type:(id -> Type0)) (#kp:key_package ip key_length key_type) (#oparam:odh_parameters{oparam.hash_length = key_length}) (op:odh_package kp oparam) (sh:share oparam) (exp:exponent oparam{exp.sh.raw_sh <> sh.raw_sh}) (h0:mem) (h1:mem) =
+let dh_op_log_change (#ip:index_package) (#key_length:(n:nat{n<=32})) (#key_type:(inst_id -> Type0)) (#kp:key_package ip key_length key_type) (#oparam:odh_parameters{oparam.hash_length = key_length}) (op:odh_package kp oparam) (sh:share oparam) (exp:exponent oparam{exp.sh.raw_sh <> sh.raw_sh}) (h0:mem) (h1:mem) =
   let i = compose_id (PK_id sh.raw_sh) (PK_id exp.sh.raw_sh) in
   let both_honest = honest ip i in
   contains h0 op.kp_log
@@ -141,7 +148,7 @@ let dh_op_log_change (#rgn:erid) (#ip:index_package rgn) (#key_length:(n:nat{n<=
       sel h1 op.kp_log == sel h0 op.kp_log)
 
 // Do we need/want this?
-let dh_op_functional_spec (#rgn:erid) (#ip:index_package rgn) (#key_length:(n:nat{n<=32})) (#key_type:(id -> Type0)) (#kp:key_package ip key_length key_type) (#oparam:odh_parameters{oparam.hash_length = key_length}) (op:odh_package kp oparam) (sh:share oparam) (exp:exponent oparam{exp.sh.raw_sh <> sh.raw_sh}) (k:key_type (compose_id (PK_id sh.raw_sh) (PK_id exp.sh.raw_sh))) (h1:mem) =
+let dh_op_functional_spec (#ip:index_package) (#key_length:(n:nat{n<=32})) (#key_type:(inst_id -> Type0)) (#kp:key_package ip key_length key_type) (#oparam:odh_parameters{oparam.hash_length = key_length}) (op:odh_package kp oparam) (sh:share oparam) (exp:exponent oparam{exp.sh.raw_sh <> sh.raw_sh}) (k:key_type (compose_id (PK_id sh.raw_sh) (PK_id exp.sh.raw_sh))) (h1:mem) =
   let i = compose_id (PK_id sh.raw_sh) (PK_id exp.sh.raw_sh) in
   let both_honest = honest ip i in
     ((Flags.prf_odh /\ both_honest) ==>
@@ -156,7 +163,7 @@ let dh_op_functional_spec (#rgn:erid) (#ip:index_package rgn) (#key_length:(n:na
 
 
 #set-options "--z3rlimit 300 --max_ifuel 2 --max_fuel 1"
-val dh_op: (#rgn:erid) -> (#ip:index_package rgn) ->  (#key_length:(n:nat{n<=32})) -> (#key_type:(id -> Type0)) -> (#kp:key_package ip key_length key_type) -> (#oparam:odh_parameters{oparam.hash_length = key_length}) -> op:odh_package kp oparam -> sh:share oparam -> exp:exponent oparam{exp.sh.raw_sh <> sh.raw_sh} -> ST (key_type (compose_id (PK_id sh.raw_sh) (PK_id exp.sh.raw_sh)))
+val dh_op: (#ip:index_package) ->  (#key_length:(n:nat{n<=32})) -> (#key_type:(inst_id -> Type0)) -> (#kp:key_package ip key_length key_type) -> (#oparam:odh_parameters{oparam.hash_length = key_length}) -> op:odh_package kp oparam -> sh:share oparam -> exp:exponent oparam{exp.sh.raw_sh <> sh.raw_sh} -> ST (key_type (compose_id (PK_id sh.raw_sh) (PK_id exp.sh.raw_sh)))
   (requires (fun h0 ->
     let i = compose_id (PK_id sh.raw_sh) (PK_id exp.sh.raw_sh) in
     (kp.flag ==> Flags.prf_odh)
