secure_api/box/Box.PKAE.fst
@@ -20,17 +20,15 @@ assume val random_bytes: n:nat -> lbytes n
 //
 //assume val pkae_flag: bool
 
-val enc_star: n:(n:nat{AE_Spec.valid_plain_length n}) -> b:lbytes (n+16){AE_Spec.valid_cipher_length (n+16)}
-let enc_star n = Seq.append (random_bytes n) (random_bytes 16)
+val ae_enc_star: n:(n:nat{AE_Spec.valid_plain_length n}) -> b:lbytes (n+16){AE_Spec.valid_cipher_length (n+16)}
+let ae_enc_star n = Seq.append (random_bytes n) (random_bytes 16)
 
-#set-options "--z3rlimit 300 --max_ifuel 2 --max_fuel 2"
 // For some reason it doesn't verify if there is an additional refinement on the output of secretbox_open_easy
 let secretbox_scheme =
-  AE.ES #(AE_Spec.keylen) #(AE_Spec.noncelen) (AE_Spec.valid_plain_length) (AE_Spec.valid_cipher_length) (fun () -> random_bytes 32) AE_Spec.secretbox_easy (enc_star) AE_Spec.secretbox_open_easy
+  AE.ES #(AE_Spec.keylen) #(AE_Spec.noncelen) (AE_Spec.valid_plain_length) (AE_Spec.valid_cipher_length) (fun () -> random_bytes 32) AE_Spec.secretbox_easy (ae_enc_star) AE_Spec.secretbox_open_easy
 
 let ae_params = AE.GP AE_Spec.keylen AE_Spec.noncelen secretbox_scheme
 
-let pp = PP (Flags.pkae) (fun n -> n / Spec.Salsa20.blocklen < pow2 32)
 
 
 //let ae_package_log_key = i:ODH.id
@@ -46,218 +44,268 @@ let hsalsa20_hash input = H.hsalsa20 input zero_nonce
 
 let odh_params = ODH.OP (ODH_Spec.serialized_point_length) (ODH_Spec.scalar_length) (H.keylen) (ODH_Spec.base_point) (ODH_Spec.scalarmult) (hsalsa20_hash)
 
-
-noeq abstract type pkae_package (rgn:erid) =
+#set-options "--z3rlimit 30 --max_ifuel 1 --max_fuel 0"
+noeq abstract type pkae_package =
   | PKAE_P :
-    pkae_rgn:erid{extends pkae_rgn rgn} ->
-    ip: index_package pkae_rgn ->
+    pkae_rgn:erid ->
+    ip: index_package ->
+    pp: plain_package{pp.flag == Flags.pkae /\ pp.valid_length == AE_Spec.valid_plain_length} ->
     kp: Key.key_package ip AE_Spec.keylen (AE.key AE_Spec.keylen) ->
-    op: ODH.odh_package #pkae_rgn #ip #AE_Spec.keylen #(AE.key AE_Spec.keylen) kp odh_params ->
-    pkae_package rgn
+    op: ODH.odh_package #ip #AE_Spec.keylen #(AE.key AE_Spec.keylen) kp odh_params ->
+    ap: AE.ae_package kp ae_params{AE.get_ap_pp ap == pp} ->
+    pkae_package
 
-let ip = create_index_package
-
-val create_pkae_package: rgn:erid -> ST pkae_package
-  (requires (fun h0 -> True))
-  (ensures (fun h0 pkae_p h1 ->
-    modifies (Set.singleton rgn) h0 h1
-    /\ extends (ODH.get_op_rgn pkae_p.op) pkae_p.op_rgn
-  ))
+#set-options "--z3rlimit 30 --max_ifuel 1 --max_fuel 0"
 let create_pkae_package rgn =
   let pkae_rgn = new_region rgn in
-  let odh_rgn = new_region pkae_rgn in
-  let op = ODH.create_odh_package kp odh_params odh_rgn in
-  let ap_log_rgn = new_region pkae_rgn in
-  let ap_rgn = new_region pkae_rgn in
-  let ap_log = MM.alloc #ap_log_rgn #ae_package_log_key #(ae_package_log_range ap_rgn) #(ae_package_log_inv ap_rgn) in
-  PKAE_P odh_rgn op ap_log_rgn ap_rgn ap_log
+  let ip = create_index_package pkae_rgn in
+  let pp = PP Flags.pkae AE_Spec.valid_plain_length in
+  let kp = AE.create_ae_key_package ip AE_Spec.keylen in
+  let op = ODH.create_odh_package pkae_rgn kp odh_params in
+  let ap = AE.create_ae_package pkae_rgn kp ae_params in
+  PKAE_P pkae_rgn ip pp kp op ap
 
 let pkey = ODH.share odh_params
+let get_pkey_raw = ODH.get_share_raw
+let get_pkey_id pk = PK_id (ODH.get_share_raw pk)
+
 let skey = ODH.exponent odh_params
+let get_skey_raw = ODH.get_exponent_raw
+let get_pkey_raw_from_skey_raw skey_raw = odh_params.ODH.exponentiate skey_raw odh_params.ODH.generator
+let get_pkey_from_skey = ODH.get_exp_share
+let get_skey_id sk = get_pkey_id (ODH.get_exp_share sk)
+
+//let nonce = AE.nonce ae_params
+//let ciphertext = AE.ciphertext ae_params
+
+let get_index_package pkae_p = pkae_p.ip
+
+let gen_footprint pkae_p h0 h1 = ODH.gen_dh_footprint pkae_p.ip odh_params h0 h1
+
+let gen pkae_p = ODH.gen_dh pkae_p.ip odh_params
+
+let coerce_pkey_footprint pkae_p pk_raw h0 h1 = ODH.coerce_dh_sh_footprint pkae_p.ip odh_params pk_raw h0 h1
+
+let coerce_pkey pkae_p pk_raw =
+  let pk = ODH.coerce_dh_sh pkae_p.ip odh_params pk_raw in
+  pk
+
+let coerce_skey_footprint pkae_p sk_raw h0 h1 = ODH.coerce_dh_exp_footprint pkae_p.ip odh_params sk_raw h0 h1
+
+let coerce_skey pkae_p sk_raw =
+  let sk = ODH.coerce_dh_exp pkae_p.ip odh_params sk_raw in
+  sk
+
+let compose_ids pk1 pk2 = compose_id (pk1) pk2
+
 let nonce = AE.nonce ae_params
 let ciphertext = AE.ciphertext ae_params
-let gen = ODH.gen_dh odh_params
 
-#set-options "--z3rlimit 300 --max_ifuel 0 --max_fuel 0"
-val get_ap_from_log: pkae_p:pkae_package -> i:ODH.id -> ST (option (ap:ae_package_log_value pkae_p.ap_rgn i))
-  (requires (fun h0 -> True))
-  (ensures (fun h0 ap h1 ->
-    (match sel h0 pkae_p.ap_log i with
-      | Some ap ->
-        contains h1 (AE.get_ap_log ap)
-        /\ MM.defined pkae_p.ap_log i h1
-        /\ MM.contains pkae_p.ap_log i ap h1
-        /\ witnessed (MM.defined pkae_p.ap_log i)
-        /\ witnessed (MM.contains pkae_p.ap_log i ap)
-      | None -> MM.fresh pkae_p.ap_log i h1)
-    /\ h0 == h1
-    /\ ap == MM.sel (sel h1 pkae_p.ap_log) i
-  ))
+let valid_ciphertext_length = AE_Spec.valid_cipher_length
 
-let get_ap_from_log pkae_p i =
-  match MM.lookup pkae_p.ap_log i with
-  | Some ap ->
-    AE.recall_log ap;
-    Some ap
-  | None -> None
+let compatible_keys pk sk = get_pkey_from_skey sk <> pk
+
+//#set-options "--z3rlimit 5 --max_ifuel 0 --max_fuel 0"
+//val create_key : pkae_p:pkae_package -> i:inst_id -> message_log_value i
+//let create_key pkae_p i =
+//  //assert(protected_plain pp i == AE.message_log_value pp i);
+//  //assert(protected_plain pp i == message_log_value i);
+//  let (ae_value : AE.message_log_value pp i) = coerce pkae_p.ip i (AE.zero_bytes (fun n -> true) 5) in
+//  admit()
+//  //let pkae_value : message_log_value i = ae_value in
+//  //pkae_value
+
+let get_log_rgn pkae_p = AE.get_log_rgn pkae_p.ap
+
+let get_pp pkae_p = AE.get_ap_pp pkae_p.ap
+
+#set-options "--z3rlimit 100 --max_ifuel 2 --max_fuel 0"
+//val get_log: pkae_p:pkae_package -> GTot (AE.ae_message_log ae_params (AE.get_ap_pp pkae_p.ap) (AE.get_log_rgn pkae_p.ap))
+//val get_log: pkae_p:pkae_package -> GTot (AE.ae_message_log ae_params (AE.get_ap_pp pkae_p.ap) (AE.get_log_rgn pkae_p.ap))
+let get_log pkae_p =
+  AE.get_ap_log pkae_p.ap
 
 
 //#set-options "--z3rlimit 300 --max_ifuel 0 --max_fuel 0"
-//val nonce_freshness_framing_lemma: pkae_p:pkae_package -> i:ODH.id -> n:nonce -> h0:mem -> h1:mem -> Lemma
-//  (requires (
-//    //((modifies (Set.singleton (ODH.get_op_rgn pkae_p.op)) h0 h1 /\ (extends (ODH.get_op_rgn pkae_p.op) pkae_p.op_rgn)) \/ h0 == h1)
-//    (modifies (Set.singleton (ODH.get_op_rgn pkae_p.op)) h0 h1 \/ h0 == h1)
-//    /\ extends (ODH.get_op_rgn pkae_p.op) pkae_p.op_rgn
-//    /\ disjoint (ODH.get_op_rgn pkae_p.op) pkae_p.ap_log_rgn
-//    /\ contains h0 pkae_p.ap_log
-//    /\ (match sel h0 pkae_p.ap_log i with
-//      | Some ap -> contains h0 (AE.get_ap_log ap)
-//      | None -> True)
+//val get_ap_from_log: pkae_p:pkae_package -> i:ODH.id -> ST (option (ap:ae_package_log_value pkae_p.ap_rgn i))
+//  (requires (fun h0 -> True))
+//  (ensures (fun h0 ap h1 ->
+//    (match sel h0 pkae_p.ap_log i with
+//      | Some ap ->
+//        contains h1 (AE.get_ap_log ap)
+//        /\ MM.defined pkae_p.ap_log i h1
+//        /\ MM.contains pkae_p.ap_log i ap h1
+//        /\ witnessed (MM.defined pkae_p.ap_log i)
+//        /\ witnessed (MM.contains pkae_p.ap_log i ap)
+//      | None -> MM.fresh pkae_p.ap_log i h1)
+//    /\ h0 == h1
+//    /\ ap == MM.sel (sel h1 pkae_p.ap_log) i
 //  ))
-//  (ensures (
-//    contains h1 pkae_p.ap_log
-//    /\ (match sel h0 pkae_p.ap_log i with
-//      | Some ap_old ->
-//        let ap_new = Some?.v (sel h1 pkae_p.ap_log i) in
-//        AE.get_ap_log ap_old == AE.get_ap_log ap_new
-//        /\ contains h1 (AE.get_ap_log ap_new)
-//      | None -> True)
-//    ///\ (let ap_option_new = sel h1 pkae_p.ap_log i in
-//    //ap_option_new == ap_option_old
-//    ///\ (Some? ap_option_new)
-//    ///\ AE.get_ap_log (Some?.v ap_option_new) == AE.get_ap_log (Some?.v ap_option_old))
+//
+//let get_ap_from_log pkae_p i =
+//  match MM.lookup pkae_p.ap_log i with
+//  | Some ap ->
+//    AE.recall_log ap;
+//    Some ap
+//  | None -> None
+//
+//
+////#set-options "--z3rlimit 300 --max_ifuel 0 --max_fuel 0"
+////val nonce_freshness_framing_lemma: pkae_p:pkae_package -> i:ODH.id -> n:nonce -> h0:mem -> h1:mem -> Lemma
+////  (requires (
+////    //((modifies (Set.singleton (ODH.get_op_rgn pkae_p.op)) h0 h1 /\ (extends (ODH.get_op_rgn pkae_p.op) pkae_p.op_rgn)) \/ h0 == h1)
+////    (modifies (Set.singleton (ODH.get_op_rgn pkae_p.op)) h0 h1 \/ h0 == h1)
+////    /\ extends (ODH.get_op_rgn pkae_p.op) pkae_p.op_rgn
+////    /\ disjoint (ODH.get_op_rgn pkae_p.op) pkae_p.ap_log_rgn
+////    /\ contains h0 pkae_p.ap_log
+////    /\ (match sel h0 pkae_p.ap_log i with
+////      | Some ap -> contains h0 (AE.get_ap_log ap)
+////      | None -> True)
+////  ))
+////  (ensures (
+////    contains h1 pkae_p.ap_log
+////    /\ (match sel h0 pkae_p.ap_log i with
+////      | Some ap_old ->
+////        let ap_new = Some?.v (sel h1 pkae_p.ap_log i) in
+////        AE.get_ap_log ap_old == AE.get_ap_log ap_new
+////        /\ contains h1 (AE.get_ap_log ap_new)
+////      | None -> True)
+////    ///\ (let ap_option_new = sel h1 pkae_p.ap_log i in
+////    //ap_option_new == ap_option_old
+////    ///\ (Some? ap_option_new)
+////    ///\ AE.get_ap_log (Some?.v ap_option_new) == AE.get_ap_log (Some?.v ap_option_old))
+////  ))
+////let nonce_freshness_framing_lemma pkae_p i n h0 h1 = ()
+//
+//#set-options "--z3rlimit 300 --max_ifuel 0 --max_fuel 0"
+//val encrypt: pkae_package:pkae_package -> pk:pkey -> sk:skey{ODH.get_share_raw pk <> ODH.get_share_raw (ODH.get_exp_share sk)} -> n:nonce -> p:protected_plain pp (ODH.create_id pk (ODH.get_exp_share sk)) -> ST ciphertext
+//  (requires (fun h0 ->
+//    let i = ODH.create_id pk (ODH.get_exp_share sk) in
+//    match sel h0 pkae_package.ap_log i with
+//    | Some ap ->
+//      contains h0 (AE.get_ap_log ap)
+//      /\ AE.nonce_is_unique ap n h0
+//    | None -> True
 //  ))
-//let nonce_freshness_framing_lemma pkae_p i n h0 h1 = ()
-
-#set-options "--z3rlimit 300 --max_ifuel 0 --max_fuel 0"
-val encrypt: pkae_package:pkae_package -> pk:pkey -> sk:skey{ODH.get_share_raw pk <> ODH.get_share_raw (ODH.get_exp_share sk)} -> n:nonce -> p:protected_plain pp (ODH.create_id pk (ODH.get_exp_share sk)) -> ST ciphertext
-  (requires (fun h0 ->
-    let i = ODH.create_id pk (ODH.get_exp_share sk) in
-    match sel h0 pkae_package.ap_log i with
-    | Some ap ->
-      contains h0 (AE.get_ap_log ap)
-      /\ AE.nonce_is_unique ap n h0
-    | None -> True
-  ))
-  (ensures (fun h0 c h1 ->
-    let i = ODH.create_id pk (ODH.get_exp_share sk) in
-    let both_honest = ODH.exp_hon sk && ODH.sh_hon pk in
-    let kp_log = ODH.get_op_log pkae_package.op in
-    // Describe ap_log state
-    Some? (sel h1 pkae_package.ap_log i)
-    /\ (let ap = Some?.v (sel h1 pkae_package.ap_log i) in
-    (if Some? (sel h0 pkae_package.ap_log i) then
-      sel h1 pkae_package.ap_log == sel h0 pkae_package.ap_log
-      /\ sel h1 (AE.get_ap_log ap) == MM.upd (sel h0 (AE.get_ap_log ap)) (n,c) p
-    else
-      sel h1 pkae_package.ap_log == MM.upd (sel h0 pkae_package.ap_log) i ap
-      /\ (forall n' . n' =!= n ==> AE.nonce_is_unique ap n' h1))
-    // Describe modified memory regions
-    /\ (let modified_regions_ap_op = Set.union
-        (AE.encrypt_modified_regions ap)
-        (ODH.dh_op_modified_regions pkae_package.op pk sk h0)
-      in
-      let modified_regions_extend_ap_log = Set.union (Set.singleton pkae_package.ap_rgn) (Set.singleton pkae_package.ap_log_rgn) in
-      let modified_regions =
-        if Some? (sel h0 pkae_package.ap_log i) then
-          modified_regions_ap_op
-        else
-          Set.union modified_regions_ap_op modified_regions_extend_ap_log
-      in
-      modifies modified_regions h0 h1)
-    /\ ODH.dh_op_log_change pkae_package.op pk sk h0 h1
-    // Describe functionality
-    /\ (let k =
-        if both_honest && ODH.get_flag() then
-          Some?.v (MM.sel (sel h1 (ODH.get_op_log pkae_package.op)) i)
-        else
-          ODH.(odh_params.hash (odh_params.exponentiate (ODH.get_exponent_raw sk) (ODH.get_share_raw pk)))
-      in
-      ODH.dh_op_functional_spec pkae_package.op pk sk k h1
-    )
-    /\ ((both_honest /\ ODH.get_flag()) ==>
-        (let k = Some?.v (MM.sel (sel h1 (ODH.get_op_log pkae_package.op)) i) in
-        AE.encrypt_functional_spec ap k n c p)
-      )
-      // In case we have a dishonest key or we don't idealize, we can't guarantee anything.
-    )
-  ))
-
-#set-options "--z3rlimit 300 --max_ifuel 0 --max_fuel 0"
-let encrypt pkae_package pk sk n p =
-  let i = ODH.create_id pk (ODH.get_exp_share sk) in
-  recall pkae_package.ap_log;
-  let k = ODH.dh_op pkae_package.op pk sk in
-  let h1 = get() in
-  ODH.recall_op_log pkae_package.op;
-  let ap =
-    match get_ap_from_log pkae_package i with
-    | Some ap ->
-      ap
-    | None ->
-      let ap = AE.create_ae_package pkae_package.ap_rgn kp ae_params pp in
-      MM.extend pkae_package.ap_log i ap;
-      ap
-  in
-  let c = AE.encrypt ap k n p in
-  //assert(
-  //    let both_honest = ODH.exp_hon sk && ODH.sh_hon pk in
-  //    (both_honest /\ ODH.get_flag()) ==>
-  //      (let k' = Some?.v (MM.sel (sel h1 (ODH.get_op_log pkae_package.op)) i) in
-  //      AE.encrypt_functional_spec ap k n c p
-  //      )
-  //    );
-  //    admit();
-  //assert(AE.encrypt_functional_spec ap k n c p);
-  c
-
-val decrypt: pkae_package:pkae_package -> pk:pkey -> sk:skey{ODH.get_share_raw pk <> ODH.get_share_raw (ODH.get_exp_share sk)} -> n:nonce -> c:ciphertext -> ST (option (p:protected_plain pp (ODH.create_id pk (ODH.get_exp_share sk))))
-  (requires (fun h0 ->
-    let i = ODH.create_id pk (ODH.get_exp_share sk) in
-    match sel h0 pkae_package.ap_log i with
-    | Some ap ->
-      contains h0 (AE.get_ap_log ap)
-    | None -> True
-  ))
-  (ensures (fun h0 c h1 ->
-    let i = ODH.create_id pk (ODH.get_exp_share sk) in
-    let both_honest = ODH.exp_hon sk && ODH.sh_hon pk in
-    let kp_log = ODH.get_op_log pkae_package.op in
-    match sel h0 pkae_package.ap_log i with
-    | Some ap ->
-      ((both_honest /\ ODH.get_flag()) ==>
-        (MM.defined kp_log i h0 ==>
-          h0 == h1)
-        /\ (MM.fresh kp_log i h0 ==>
-          modifies (Set.singleton (ODH.get_op_rgn pkae_package.op)) h0 h1))
-      /\ ((~both_honest \/ ~(ODH.get_flag())) ==>
-          h0 == h1)
-    | None ->
-      MM.defined pkae_package.ap_log i h1
-      /\ (let ap = Some?.v (sel h1 pkae_package.ap_log i) in
-        sel h1 pkae_package.ap_log == MM.upd (sel h0 pkae_package.ap_log) i ap
-        /\ ((both_honest /\ ODH.get_flag()) ==>
-            (MM.defined kp_log i h0 ==>
-              modifies (Set.union (Set.singleton pkae_package.ap_rgn) (Set.singleton pkae_package.ap_log_rgn)) h0 h1)
-            /\ (MM.fresh kp_log i h0 ==>
-              modifies (Set.union (Set.singleton pkae_package.ap_rgn) (Set.union (Set.singleton pkae_package.ap_log_rgn) (Set.singleton (ODH.get_op_rgn pkae_package.op)))) h0 h1))
-        /\ ((~both_honest \/ ~(ODH.get_flag())) ==>
-            (modifies (Set.union (Set.singleton pkae_package.ap_rgn) (Set.singleton pkae_package.ap_log_rgn)) h0 h1)))
-  ))
-
-let decrypt pkae_package pk sk n c =
-  let i = ODH.create_id pk (ODH.get_exp_share sk) in
-  recall pkae_package.ap_log;
-  let k = ODH.dh_op pkae_package.op pk sk in
-  let ap =
-    match get_ap_from_log pkae_package i with
-    | Some ap ->
-      ap
-    | None ->
-      let ap = AE.create_ae_package pkae_package.ap_rgn kp ae_params pp in
-      MM.extend pkae_package.ap_log i ap;
-      recall pkae_package.ap_log;
-      AE.recall_log ap;
-      ap
-  in
-  AE.decrypt ap k n c
+//  (ensures (fun h0 c h1 ->
+//    let i = ODH.create_id pk (ODH.get_exp_share sk) in
+//    let both_honest = ODH.exp_hon sk && ODH.sh_hon pk in
+//    let kp_log = ODH.get_op_log pkae_package.op in
+//    // Describe ap_log state
+//    Some? (sel h1 pkae_package.ap_log i)
+//    /\ (let ap = Some?.v (sel h1 pkae_package.ap_log i) in
+//    (if Some? (sel h0 pkae_package.ap_log i) then
+//      sel h1 pkae_package.ap_log == sel h0 pkae_package.ap_log
+//      /\ sel h1 (AE.get_ap_log ap) == MM.upd (sel h0 (AE.get_ap_log ap)) (n,c) p
+//    else
+//      sel h1 pkae_package.ap_log == MM.upd (sel h0 pkae_package.ap_log) i ap
+//      /\ (forall n' . n' =!= n ==> AE.nonce_is_unique ap n' h1))
+//    // Describe modified memory regions
+//    /\ (let modified_regions_ap_op = Set.union
+//        (AE.encrypt_modified_regions ap)
+//        (ODH.dh_op_modified_regions pkae_package.op pk sk h0)
+//      in
+//      let modified_regions_extend_ap_log = Set.union (Set.singleton pkae_package.ap_rgn) (Set.singleton pkae_package.ap_log_rgn) in
+//      let modified_regions =
+//        if Some? (sel h0 pkae_package.ap_log i) then
+//          modified_regions_ap_op
+//        else
+//          Set.union modified_regions_ap_op modified_regions_extend_ap_log
+//      in
+//      modifies modified_regions h0 h1)
+//    /\ ODH.dh_op_log_change pkae_package.op pk sk h0 h1
+//    // Describe functionality
+//    /\ (let k =
+//        if both_honest && ODH.get_flag() then
+//          Some?.v (MM.sel (sel h1 (ODH.get_op_log pkae_package.op)) i)
+//        else
+//          ODH.(odh_params.hash (odh_params.exponentiate (ODH.get_exponent_raw sk) (ODH.get_share_raw pk)))
+//      in
+//      ODH.dh_op_functional_spec pkae_package.op pk sk k h1
+//    )
+//    /\ ((both_honest /\ ODH.get_flag()) ==>
+//        (let k = Some?.v (MM.sel (sel h1 (ODH.get_op_log pkae_package.op)) i) in
+//        AE.encrypt_functional_spec ap k n c p)
+//      )
+//      // In case we have a dishonest key or we don't idealize, we can't guarantee anything.
+//    )
+//  ))
+//
+//#set-options "--z3rlimit 300 --max_ifuel 0 --max_fuel 0"
+//let encrypt pkae_package pk sk n p =
+//  let i = ODH.create_id pk (ODH.get_exp_share sk) in
+//  recall pkae_package.ap_log;
+//  let k = ODH.dh_op pkae_package.op pk sk in
+//  let h1 = get() in
+//  ODH.recall_op_log pkae_package.op;
+//  let ap =
+//    match get_ap_from_log pkae_package i with
+//    | Some ap ->
+//      ap
+//    | None ->
+//      let ap = AE.create_ae_package pkae_package.ap_rgn kp ae_params pp in
+//      MM.extend pkae_package.ap_log i ap;
+//      ap
+//  in
+//  let c = AE.encrypt ap k n p in
+//  //assert(
+//  //    let both_honest = ODH.exp_hon sk && ODH.sh_hon pk in
+//  //    (both_honest /\ ODH.get_flag()) ==>
+//  //      (let k' = Some?.v (MM.sel (sel h1 (ODH.get_op_log pkae_package.op)) i) in
+//  //      AE.encrypt_functional_spec ap k n c p
+//  //      )
+//  //    );
+//  //    admit();
+//  //assert(AE.encrypt_functional_spec ap k n c p);
+//  c
+//
+//val decrypt: pkae_package:pkae_package -> pk:pkey -> sk:skey{ODH.get_share_raw pk <> ODH.get_share_raw (ODH.get_exp_share sk)} -> n:nonce -> c:ciphertext -> ST (option (p:protected_plain pp (ODH.create_id pk (ODH.get_exp_share sk))))
+//  (requires (fun h0 ->
+//    let i = ODH.create_id pk (ODH.get_exp_share sk) in
+//    match sel h0 pkae_package.ap_log i with
+//    | Some ap ->
+//      contains h0 (AE.get_ap_log ap)
+//    | None -> True
+//  ))
+//  (ensures (fun h0 c h1 ->
+//    let i = ODH.create_id pk (ODH.get_exp_share sk) in
+//    let both_honest = ODH.exp_hon sk && ODH.sh_hon pk in
+//    let kp_log = ODH.get_op_log pkae_package.op in
+//    match sel h0 pkae_package.ap_log i with
+//    | Some ap ->
+//      ((both_honest /\ ODH.get_flag()) ==>
+//        (MM.defined kp_log i h0 ==>
+//          h0 == h1)
+//        /\ (MM.fresh kp_log i h0 ==>
+//          modifies (Set.singleton (ODH.get_op_rgn pkae_package.op)) h0 h1))
+//      /\ ((~both_honest \/ ~(ODH.get_flag())) ==>
+//          h0 == h1)
+//    | None ->
+//      MM.defined pkae_package.ap_log i h1
+//      /\ (let ap = Some?.v (sel h1 pkae_package.ap_log i) in
+//        sel h1 pkae_package.ap_log == MM.upd (sel h0 pkae_package.ap_log) i ap
+//        /\ ((both_honest /\ ODH.get_flag()) ==>
+//            (MM.defined kp_log i h0 ==>
+//              modifies (Set.union (Set.singleton pkae_package.ap_rgn) (Set.singleton pkae_package.ap_log_rgn)) h0 h1)
+//            /\ (MM.fresh kp_log i h0 ==>
+//              modifies (Set.union (Set.singleton pkae_package.ap_rgn) (Set.union (Set.singleton pkae_package.ap_log_rgn) (Set.singleton (ODH.get_op_rgn pkae_package.op)))) h0 h1))
+//        /\ ((~both_honest \/ ~(ODH.get_flag())) ==>
+//            (modifies (Set.union (Set.singleton pkae_package.ap_rgn) (Set.singleton pkae_package.ap_log_rgn)) h0 h1)))
+//  ))
+//
+//let decrypt pkae_package pk sk n c =
+//  let i = ODH.create_id pk (ODH.get_exp_share sk) in
+//  recall pkae_package.ap_log;
+//  let k = ODH.dh_op pkae_package.op pk sk in
+//  let ap =
+//    match get_ap_from_log pkae_package i with
+//    | Some ap ->
+//      ap
+//    | None ->
+//      let ap = AE.create_ae_package pkae_package.ap_rgn kp ae_params pp in
+//      MM.extend pkae_package.ap_log i ap;
+//      recall pkae_package.ap_log;
+//      AE.recall_log ap;
+//      ap
+//  in
+//  AE.decrypt ap k n c
