secure_api/box/Box.PKAE.fsti
@@ -9,126 +9,161 @@ open FStar.Endianness
 
 open Box.Plain
 open Box.Index
+open Mem
 
 module MM = FStar.Monotonic.Map
 
-let n32 = (n:nat{n<=32})
+let n32 = nat
 let bytes32 = b:bytes{Seq.length b <= 32}
 
-#set-options "--z3rlimit 300 --max_ifuel 1 --max_fuel 1"
-
-val pp : (pp:plain_package{pp.flag == Flags.pkae})
-
+val pkae_package: Type u#1
 // Footpring function instead of rgn in the type
-val pkae_package: rgn:erid -> Type u#1
+//val pkae_package: rgn:erid -> Type0
 
-//val create_pkae_package: rgn:erid -> ST (pkae_package rgn)
-//  (requires (fun h0 -> True))
-//  (ensures (fun h0 pkae_p h1 ->
-//    modifies (Set.singleton rgn) h0 h1
-//  ))
-//
-////val pkey_length: n32
-//let pkey_length = 32
-//val pkey : Type
-//val get_pkey_raw: pkey -> Tot (lbytes pkey_length)
-//val get_pkey_id: pk:pkey -> Tot (i:pk_id{i = PK_id (get_pkey_raw pk)})
-//
-////val skey_length: n32
-//let skey_length = 32
-//val skey : Type
-//val get_skey_raw: skey -> GTot (lbytes pkey_length)
-//val get_pkey_from_skey: skey -> pkey
-//val get_skey_id: sk:skey -> Tot (i:pk_id{i = PK_id (get_pkey_raw (get_pkey_from_skey sk))})
-//
-//val gen : #rgn:erid -> ip:index_package rgn -> ST (keypair:(pkey*skey))
-//  (requires (fun h0 -> True))
-//  (ensures (fun h0 keypair h1 ->
-//    get_pkey_from_skey (snd keypair) == fst keypair
-//    /\ honest ip (PK_id (get_pkey_raw (fst keypair)))
-//    /\ modifies (Set.singleton rgn) h0 h1
-//  ))
-//
-//val coerce : #rgn:erid -> ip:index_package rgn -> pk_raw:lbytes pkey_length -> sk_raw:lbytes skey_length ->ST (keypair:(pkey*skey))
-//  (requires (fun h0 ->
-//    fresh ip (PK_id pk_raw) h0
-//  ))
-//  (ensures (fun h0 keypair h1 ->
-//    get_pkey_from_skey (snd keypair) == fst keypair
-//    /\ dishonest ip (get_pkey_id (fst keypair))
-//    /\ get_pkey_raw (fst keypair) = pk_raw
-//    /\ get_skey_raw (snd keypair) = sk_raw
-//    /\ modifies (Set.singleton rgn) h0 h1
-//  ))
-//
-//val compose_ids: pk_id -> pk_id -> inst_id
-//
-//val nonce_length:n32
-//let nonce = lbytes nonce_length
+val create_pkae_package: rgn:erid -> ST (pkae_package)
+  (requires (fun h0 -> True))
+  (ensures (fun h0 pkae_p h1 ->
+    modifies (Set.singleton rgn) h0 h1
+  ))
+
+//val pkey_length: n32
+let pkey_length = 32
+val pkey : Type0
+val get_pkey_raw: pkey -> Tot (lbytes pkey_length)
+val get_pkey_id: pk:pkey -> Tot (i:pk_id{i = PK_id (get_pkey_raw pk)})
+
+//val skey_length: n32
+let skey_length = 32
+val skey : Type0
+val get_skey_raw: skey -> GTot (lbytes pkey_length)
+val get_pkey_raw_from_skey_raw: lbytes skey_length -> lbytes pkey_length
+val get_pkey_from_skey: sk:skey -> pk:pkey{get_pkey_raw pk = get_pkey_raw_from_skey_raw (get_skey_raw sk)}
+val get_skey_id: sk:skey -> Tot (i:pk_id{i = PK_id (get_pkey_raw (get_pkey_from_skey sk))})
+
+
+val get_index_package: pkae_p:pkae_package -> ip:index_package
+
+let honest pkae_p i = honest (get_index_package pkae_p) i
+let dishonest pkae_p i = dishonest (get_index_package pkae_p) i
+let registered pkae_p i = registered (get_index_package pkae_p) i
+let fresh pkae_p i h = fresh (get_index_package pkae_p) i h
+
+val gen_footprint: pkae_package -> h0:mem -> h1:mem -> Type0
+
+val gen : pkae_p:pkae_package -> ST (keypair:(skey*pkey))
+  (requires (fun h0 -> True))
+  (ensures (fun h0 keypair h1 ->
+    get_pkey_from_skey (fst keypair) == snd keypair
+    /\ honest pkae_p (get_pkey_id (snd keypair))
+    /\ gen_footprint pkae_p h0 h1
+  ))
+
+val coerce_pkey_footprint: pkae_package -> pk_raw:lbytes pkey_length -> h0:mem -> h1:mem -> Type0
+
+val coerce_pkey : pkae_p:pkae_package -> pk_raw:lbytes pkey_length -> ST (pk:pkey)
+  (requires (fun h0 ->
+    fresh pkae_p (PK_id pk_raw) h0
+  ))
+  (ensures (fun h0 pk h1 ->
+    dishonest pkae_p (get_pkey_id pk)
+    /\ get_pkey_raw pk = pk_raw
+    /\ coerce_pkey_footprint pkae_p pk_raw h0 h1
+  ))
+
+val coerce_skey_footprint: pkae_package -> sk_raw:lbytes skey_length -> h0:mem -> h1:mem -> Type0
+
+val coerce_skey : pkae_p:pkae_package -> sk_raw:lbytes skey_length -> ST (sk:skey)
+  (requires (fun h0 ->
+    fresh pkae_p (PK_id (get_pkey_raw_from_skey_raw sk_raw)) h0
+  ))
+  (ensures (fun h0 sk h1 ->
+    dishonest pkae_p (get_skey_id sk)
+    /\ get_skey_raw sk = sk_raw
+    /\ coerce_skey_footprint pkae_p sk_raw h0 h1
+  ))
+
+val compose_ids: pk1:pk_id -> pk2:pk_id{pk1 <> pk2} -> inst_id
+
+val nonce: eqtype
+val ciphertext: eqtype
 //val valid_ciphertext_length : n32 -> bool
 //let ciphertext = b:bytes32{valid_ciphertext_length (Seq.length b)}
+
+
+//type message_log_key = inst_id*nonce*ciphertext
+//type message_log_key = inst_id*nonce*ciphertext
+////  | LOG_KEY: i:inst_id -> n:nonce -> c:ciphertext -> message_log_key
 //
-//val compatible_keys: pkey -> skey -> bool
-//
-//type message_log_key =
-//  | LOG_KEY: i:inst_id -> n:nonce -> c:ciphertext -> message_log_key
+//let fst t = Mktuple3?._1 t
+//let snd t = Mktuple3?._2 t
+//let thrd t = Mktuple3?._3 t
 //
 //let message_log_value (i:inst_id) = protected_plain pp i
-//let message_log_range (k:message_log_key) = message_log_value (k.i)
+//let message_log_range (k:message_log_key) = message_log_value (Mktuple3?._1 k)
 //let message_log_inv (f:MM.map' (message_log_key) (message_log_range)) = True
 //
 //let message_log (rgn:erid) =
 //  MM.t rgn (message_log_key) (message_log_range) (message_log_inv)
-//
-//val get_log: #rgn:erid -> pkae_package rgn -> message_log rgn
-//
-//let nonce_is_unique (#rgn:erid) (pkae_p:pkae_package rgn) (i:inst_id) (n:nonce) (h0:mem) =
-//  forall c . MM.fresh (get_log pkae_p) (LOG_KEY i n c) h0
-//
-//let extended_message_log (#rgn:erid) (pkae_p:pkae_package rgn) (i:inst_id) (n:nonce) (c:ciphertext) (p:protected_plain pp i) (h0:mem) (h1:mem) =
-//  let log_key = LOG_KEY i n c in
-//  let log_value = p in
-//  let log = get_log pkae_p in
-//  sel h1 log == MM.upd (sel h0 log) log_key log_value
-//  /\ witnessed (MM.defined log log_key)
-//  /\ witnessed (MM.contains log log_key log_value)
-//
-//
-//val enc_spec: p:plain pp -> pk:lbytes pkey_length -> sk:lbytes skey_length -> n:nonce -> c:ciphertext
-////val enc_star: plain_length:n32 -> pk:lbytes pkey_length -> sk:lbytes skey_length -> n:nonce -> c:ciphertext
-//val dec_spec: c:ciphertext -> pk:lbytes pkey_length -> sk:lbytes skey_length -> n:nonce -> option (p:plain pp)
-//
-//#set-options "--z3rlimit 300 --max_ifuel 0 --max_fuel 0"
-//val encrypt: #rgn:erid -> pkae_p:pkae_package rgn -> ip:index_package rgn -> pk:pkey -> sk:skey{compatible_keys pk sk} -> n:nonce -> p:protected_plain pp (compose_ids (get_pkey_id pk) (get_skey_id sk)) -> ST ciphertext
-//  (requires (fun h0 ->
-//    let i = compose_ids (get_pkey_id pk) (get_skey_id sk) in
-//    nonce_is_unique pkae_p i n h0
-//  ))
-//  (ensures (fun h0 c h1 ->
-//    let i = compose_ids (get_pkey_id pk) (get_skey_id sk) in
-//    //let both_honest = honest ip i in
-//    modifies (Set.singleton rgn) h0 h1
-//    /\ ((honest ip i /\ Flags.pkae) ==>
-//      c == enc_star (length p) (get_pkey_raw pk) (get_skey_raw sk) n)
-//    /\ ((dishonest ip i \/ ~(Flags.pkae)) ==>
-//      c == enc_spec (repr #rgn #pp #ip #i p) (get_pkey_raw pk) (get_skey_raw sk) n)
-//    /\ extended_message_log pkae_p i n c p h0 h1
-//  ))
-//
-//val decrypt: #rgn:erid -> pkae_p:pkae_package rgn -> ip:index_package rgn -> pk:pkey -> sk:skey{compatible_keys pk sk} -> n:nonce -> c:ciphertext -> ST (option_p:option (protected_plain pp (compose_ids (get_pkey_id pk) (get_skey_id sk))))
-//  (requires (fun h0 ->
-//    True
-//  ))
-//  (ensures (fun h0 option_p h1 ->
-//    let i = compose_ids (get_pkey_id pk) (get_skey_id sk) in
-//    let option_spec = dec_spec c (get_pkey_raw pk) (get_skey_raw sk) n in
-//    (modifies (Set.singleton rgn) h0 h1 \/ h0 == h1)
-//    /\ ((honest ip i /\ Flags.pkae) ==>
-//      (MM.sel (sel h0 (get_log pkae_p)) (LOG_KEY i n c) == option_p)
-//      )
-//    /\ ((dishonest ip i \/ ~(Flags.pkae)) ==>
-//      (Some? option_spec ==>
-//      (Some? option_p
-//      /\ repr #rgn #pp #ip #i (Some?.v option_p) == Some?.v option_spec))
-//      )
-//  ))
+val compatible_keys: pkey -> skey -> bool
+
+val get_log_rgn: pkae_p:pkae_package -> Tot (rgn:erid)
+
+val get_pp: pkae_p:pkae_package -> plain_package
+
+val get_log: pkae_p:pkae_package -> GTot (Mem.message_log nonce ciphertext (get_pp pkae_p) (get_log_rgn pkae_p))
+//val get_log: pkae_p:pkae_package -> GTot (Mem.message_log nonce ciphertext pp (get_log_rgn pkae_p))
+
+
+//val nonce_is_unique: (pkae_p:pkae_package) -> (i:inst_id) -> (n:nonce) -> (h0:mem) -> GTot (t:Type0{t <==> (forall c . MM.fresh (get_log pkae_p) (i,n,c) h0)})
+let nonce_is_unique pkae_p i n h0 =
+  forall c . MM.fresh (get_log pkae_p) (i,n,c) h0
+
+let extended_message_log (pkae_p:pkae_package) (i:inst_id) (n:nonce) (c:ciphertext) (p:protected_plain (get_pp pkae_p) i) (h0:mem) (h1:mem) =
+  let log_key = i,n,c in
+  let log_value = p in
+  let log = get_log pkae_p in
+  sel h1 log == MM.upd (sel h0 log) log_key log_value
+  /\ witnessed (MM.defined log log_key)
+  /\ witnessed (MM.contains log log_key log_value)
+
+val encrypt_footprint: (pkae_p:pkae_package) -> (i:inst_id) -> (n:nonce) -> (c:ciphertext) -> (p:protected_plain (get_pp pkae_p) i) -> (h0:mem) -> (h1:mem) -> Type0
+val decrypt_footprint: (pkae_p:pkae_package) -> (i:inst_id) -> (n:nonce) -> (c:ciphertext) -> option (p:protected_plain (get_pp pkae_p) i) -> (h0:mem) -> (h1:mem) -> Type0
+
+val enc_spec: pkae_p:pkae_package -> p:plain (get_pp pkae_p) -> pk:lbytes pkey_length -> sk:lbytes skey_length -> n:nonce -> c:ciphertext
+val enc_star: pkae_p:pkae_package -> plain_length:n32{(get_pp pkae_p).valid_length plain_length} -> c:ciphertext
+val dec_spec: pkae_p:pkae_package -> c:ciphertext -> pk:lbytes pkey_length -> sk:lbytes skey_length -> n:nonce -> option (p:plain (get_pp pkae_p))
+
+#set-options "--z3rlimit 300 --max_ifuel 0 --max_fuel 0"
+val encrypt: pkae_p:pkae_package -> pk:pkey -> sk:skey{compatible_keys pk sk} -> n:nonce -> p:protected_plain (get_pp pkae_p) (compose_ids (get_pkey_id pk) (get_skey_id sk)) -> ST ciphertext
+  (requires (fun h0 ->
+    let i = compose_ids (get_pkey_id pk) (get_skey_id sk) in
+    nonce_is_unique pkae_p i n h0
+    /\ registered pkae_p i
+  ))
+  (ensures (fun h0 c h1 ->
+    let i = compose_ids (get_pkey_id pk) (get_skey_id sk) in
+    encrypt_footprint pkae_p i n c p h0 h1
+    /\ ((honest pkae_p i /\ Flags.pkae) ==>
+      c == enc_star pkae_p (Plain.length p))
+    /\ ((dishonest pkae_p i \/ ~(Flags.pkae)) ==>
+      c == enc_spec pkae_p (repr #(get_pp pkae_p) #(get_index_package pkae_p) #i p) (get_pkey_raw pk) (get_skey_raw sk) n)
+    /\ extended_message_log pkae_p i n c p h0 h1
+  ))
+
+val decrypt: pkae_p:pkae_package -> pk:pkey -> sk:skey{compatible_keys pk sk} -> n:nonce -> c:ciphertext -> ST (option_p:option (protected_plain (get_pp pkae_p) (compose_ids (get_pkey_id pk) (get_skey_id sk))))
+  (requires (fun h0 ->
+    True
+  ))
+  (ensures (fun h0 option_p h1 ->
+    let i = compose_ids (get_pkey_id pk) (get_skey_id sk) in
+    let option_spec = dec_spec pkae_p c (get_pkey_raw pk) (get_skey_raw sk) n in
+    decrypt_footprint pkae_p i n c option_p h0 h1
+    /\ ((honest pkae_p i /\ Flags.pkae) ==>
+      (MM.sel (sel h0 (get_log pkae_p)) (i,n,c) == option_p)
+      )
+    /\ ((dishonest pkae_p i \/ ~(Flags.pkae)) ==>
+      (Some? option_spec ==>
+      (Some? option_p
+      /\ repr #(get_pp pkae_p) #(get_index_package pkae_p) #i (Some?.v option_p) == Some?.v option_spec))
+      )
+  ))
