secure_api/box/Box.Flags.fsti
@@ -4,4 +4,4 @@ val prf_odh : b:bool
 
 val ae: b:bool{b ==> prf_odh}
 
-val pkae : b:bool{b ==> prf_odh /\ ae}
+val pkae : b:bool{b <==> prf_odh /\ ae}
