secure_api/box/Mem.fst
@@ -1,0 +1,24 @@
+module Mem
+
+open FStar.HyperStack
+open FStar.HyperStack.ST
+
+open Box.Index
+open Box.Plain
+
+
+module MM = FStar.Monotonic.Map
+
+type message_log_key (nonce:Type0) (ciphertext:Type0) = inst_id*nonce*ciphertext
+//  | LOG_KEY: i:inst_id -> n:nonce aparams -> c:ciphertext aparams -> message_log_key aparams
+
+let message_log_value (pp:plain_package) (i:inst_id) = protected_plain pp i
+let message_log_range (#nonce:Type0) (#ciphertext:Type0) (pp:plain_package)  (k:message_log_key nonce ciphertext) = message_log_value pp (Mktuple3?._1 k)
+let message_log_inv (#nonce:Type0) (#ciphertext:Type0) (#pp:plain_package) (f:MM.map' (message_log_key nonce ciphertext) (message_log_range pp)) = True
+
+let message_log (nonce:Type0) (ciphertext:Type0) (pp:plain_package) (rgn:erid) =
+  MM.t rgn (message_log_key nonce ciphertext) (message_log_range pp) (message_log_inv)
+
+let empty_message_log (nonce:Type0) (ciphertext:Type0) (pp:plain_package) = MM.empty_map (message_log_key nonce ciphertext) (message_log_range pp)
+
+let alloc_message_log (nonce:Type0) (ciphertext:Type0) (rgn:erid) (pp:plain_package) = MM.alloc #rgn #(message_log_key nonce ciphertext) #(message_log_range pp) #(message_log_inv)
